revising HSL.Transcript to allow for Handshake, 12, and 13 messages

src/tls/HSL.Common.fst
@@ -1,42 +1,45 @@
 module HSL.Common
 
 open FStar.Integers
-open FStar.HyperStack.ST
-
-module G = FStar.Ghost
-module List = FStar.List.Tot
 
 module HS = FStar.HyperStack
 module B = LowStar.Buffer
 
-module C = TLSConstants
-module Hash = Hashing
-module HashSpec = Hashing.Spec
 module HSM = Parsers.Handshake
+module HSM12 = Parsers.Handshake12
+module HSM13 = Parsers.Handshake13
 
-module LP = LowParse.Low.Base
+type bytes = LowParse.Bytes.bytes
 
-type hbytes = Spec.Hash.Definitions.bytes
-
-/// TODO: define using high-level serializers from LowParse
+#set-options "--max_fuel 0 --max_ifuel 0"
 
 [@"opaque_to_smt"]
-let format_hs_msg (m:HSM.handshake) : GTot hbytes =
+let format_hs_msg (m:HSM.handshake) : GTot bytes =
   HSM.handshake_serializer m
 
-/// TODO: LowParse definition of saying buf is a valid serialization of m
+[@"opaque_to_smt"]
+let format_hs12_msg (m:HSM12.handshake12) : GTot bytes =
+  HSM12.handshake12_serializer m
 
-let valid_parsing_aux (m:HSM.handshake) (buf:B.buffer uint_8) (h:HS.mem) =
-  format_hs_msg m == B.as_seq h buf
+[@"opaque_to_smt"]
+let format_hs13_msg (m:HSM13.handshake13) : GTot bytes =
+  HSM13.handshake13_serializer m
 
+/// Buffer [from, to) is a serialization of m
 
-#reset-options "--log_queries --max_fuel 0 --max_ifuel 0 --query_stats"
-/// Helper to enforce spatial safety of indices in the st input buffer
-/// and that the buffer is a serialization of m
 let valid_parsing (m:HSM.handshake) (from to:uint_32) (b:B.buffer uint_8) (h:HS.mem) =
-  from <= to /\
-  to <= B.len b /\
+  from <= to /\ to <= B.len b /\
   (let buf = B.gsub b from (to - from) in
-   valid_parsing_aux m buf h)
+   format_hs_msg m == B.as_seq h buf)
+
+let valid_parsing12 (m:HSM12.handshake12) (from to:uint_32) (b:B.buffer uint_8) (h:HS.mem) =
+  from <= to /\ to <= B.len b /\
+  (let buf = B.gsub b from (to - from) in
+   format_hs12_msg m == B.as_seq h buf)
+
+let valid_parsing13 (m:HSM13.handshake13) (from to:uint_32) (b:B.buffer uint_8) (h:HS.mem) =
+  from <= to /\ to <= B.len b /\
+  (let buf = B.gsub b from (to - from) in
+   format_hs13_msg m == B.as_seq h buf)
 
 let region_includes r l = B.loc_regions true (Set.singleton r) `B.loc_includes` l
