src/tls/HSL.Transcript.fst
@@ -10,23 +10,20 @@ module HS = FStar.HyperStack
 module ST = FStar.HyperStack.ST
 module B = LowStar.Buffer
 
-module Hash = Hashing
-module HSM = HandshakeMessages
+module HSM = Parsers.Handshake
+module HSM12 = Parsers.Handshake12
+module HSM13 = Parsers.Handshake13
 
 open HSL.Common
 
 module IncHash = EverCrypt.Hash.Incremental
 
-#reset-options
-   "--log_queries --query_stats \
-    --using_facts_from 'Prims FStar LowStar -FStar.Reflection -FStar.Tactics -FStar.UInt128 -FStar.Math' \
-    --using_facts_from 'Mem HSL Types_s Words_s Range Spec.Hash Hacl.Hash.Definitions' \
-    --using_facts_from 'TLSError EverCrypt'"
+#reset-options "--using_facts_from '* -FStar.Tactics -FStar.Reflection -LowParse'"
 
 noeq
 type state = {
-  rgn:Mem.rgn;
-  hash_state: B.pointer (option (a:Hash.alg & IncHash.state a));
+  rgn: Mem.rgn;
+  hash_state: B.pointer (option (a:alg & IncHash.state a));
   tx: (p:B.pointer (G.erased transcript_t){
     B.loc_disjoint (B.loc_buffer hash_state) (B.loc_buffer p)
   })
@@ -65,12 +62,12 @@ let invariant s h =
   B.live h s.hash_state /\
   B.live h s.tx /\
   (match B.deref h s.hash_state with
-   | None -> transcript s h == []
+   | None -> transcript s h == Transcript_nil
    | Some (| a, hash_st |) ->
      IncHash.hashes #a h hash_st (transcript_bytes (transcript s h)))
 
 private
-let frame_inc_hashes (#a:Hash.alg) (hash_st:IncHash.state a) (h0 h1 : HS.mem) (b:hbytes) (l:B.loc)
+let frame_inc_hashes (#a:alg) (hash_st:IncHash.state a) (h0 h1 : HS.mem) (b:bytes) (l:B.loc)
   : Lemma
     (requires
       B.loc_disjoint l (IncHash.footprint hash_st h0) /\
@@ -78,11 +75,8 @@ let frame_inc_hashes (#a:Hash.alg) (hash_st:IncHash.state a) (h0 h1 : HS.mem) (b
       IncHash.hashes #a h0 hash_st b)
     (ensures
       IncHash.hashes #a h1 hash_st b)
-  = assert (IncHash.footprint hash_st h0 == B.(loc_union (loc_buffer (hash_st.IncHash.buf))
-                                                         (EverCrypt.Hash.footprint (hash_st.IncHash.hash_state) h0)));
-    IncHash.modifies_disjoint_preserves l h0 h1 hash_st
+  = IncHash.modifies_disjoint_preserves l h0 h1 hash_st
 
-#push-options "--max_fuel 1 --initial_fuel 1 --max_ifuel 1 --initial_ifuel 1"
 module T = FStar.Tactics
 let framing s l h0 h1 =
   assert (footprint' s h0 == footprint s h0)
@@ -98,7 +92,7 @@ let framing s l h0 h1 =
 
 let create r =
   let hash_state = B.malloc r None 1ul in
-  let tx = B.malloc r (G.hide []) 1ul in
+  let tx = B.malloc r (G.hide Transcript_nil) 1ul in
   { rgn = r; hash_state = hash_state; tx = tx }
 
 let set_hash_alg a s =
@@ -116,21 +110,33 @@ let set_hash_alg a s =
   IncHash.modifies_disjoint_preserves (B.loc_buffer s.hash_state) h1 h2 hash_st;
 
   //AR: the postcondition in IncHash is in terms of Hash.fresh_loc, that needs fixing 
-  assume (B.(fresh_loc (IncHash.footprint hash_st h2) h0 h2));  
+  assume (B.(fresh_loc (IncHash.footprint hash_st h2) h0 h2))
 
-  //AR: surprising that we can't prove it ...
-  assume (B.live h2 hash_st.IncHash.buf)
+let lemma_transcript_bytes (m:HSM.handshake) (t:transcript_t)
+  : Lemma
+      (requires (can_extend_with_hsm t))
+      (ensures  (transcript_bytes (extend_transcript t m) ==
+                 Seq.append (transcript_bytes t) (format_hs_msg m)))
+  = admit ()
 
-let lemma_transcript_bytes (hd:HSM.hs_msg) (l:transcript_t)
-  : Lemma (transcript_bytes (hd::l) ==
-           Seq.append (transcript_bytes l) (format_hs_msg hd))
-  = ()
+let lemma_transcript_bytes12 (m:HSM12.handshake12) (t:transcript_t)
+  : Lemma
+      (requires (can_extend_with_hsm12 t))
+      (ensures  (transcript_bytes (extend_transcript12 t m) ==
+                 Seq.append (transcript_bytes t) (format_hs12_msg m)))
+  = admit ()
 
-#push-options "--z3rlimit_factor 4 --max_fuel 0"
+let lemma_transcript_bytes13 (m:HSM13.handshake13) (t:transcript_t)
+  : Lemma
+      (requires (can_extend_with_hsm13 t))
+      (ensures  (transcript_bytes (extend_transcript13 t m) ==
+                 Seq.append (transcript_bytes t) (format_hs13_msg m)))
+  = admit ()
+
+#set-options "--z3rlimit 40 --max_fuel 0 --max_ifuel 1 --initial_ifuel 1"
 let extend_hash s b p0 p1 msg =
   let hash_st_opt = B.index s.hash_state 0ul in
   match hash_st_opt with
-  | None -> ()
   | Some (| a, hash_st |) ->
     let e_tx = B.index s.tx 0ul in
     let prev_bytes = G.elift1 transcript_bytes e_tx in
@@ -145,7 +151,7 @@ let extend_hash s b p0 p1 msg =
 
     B.upd s.hash_state 0ul (Some (| a, new_hash_st |));
 
-    let e_tx = G.elift2 Cons msg e_tx in
+    let e_tx = G.elift2_p extend_transcript e_tx msg in
     B.upd s.tx 0ul e_tx;
 
     let h3 = ST.get () in
@@ -155,6 +161,62 @@ let extend_hash s b p0 p1 msg =
                                                      (B.loc_buffer s.tx)) h1 h3 new_hash_st;
 
     lemma_transcript_bytes (G.reveal msg) (transcript s h0)
+
+let extend_hash12 s b p0 p1 msg =
+  let hash_st_opt = B.index s.hash_state 0ul in
+  match hash_st_opt with
+  | Some (| a, hash_st |) ->
+    let e_tx = B.index s.tx 0ul in
+    let prev_bytes = G.elift1 transcript_bytes e_tx in
+    let sub_b = B.sub b p0 (p1 - p0) in
+    assume (Seq.length (G.reveal prev_bytes) + UInt32.v (p1 - p0) < pow2 61);
+
+    let h0 = ST.get () in
+
+    let new_hash_st = IncHash.update a hash_st prev_bytes sub_b (p1 - p0) in
+
+    let h1 = ST.get () in
+
+    B.upd s.hash_state 0ul (Some (| a, new_hash_st |));
+
+    let e_tx = G.elift2_p extend_transcript12 e_tx msg in
+    B.upd s.tx 0ul e_tx;
+
+    let h3 = ST.get () in
+
+    //AR: this does not have a pattern, so need to call explicitly
+    IncHash.modifies_disjoint_preserves (B.loc_union (B.loc_buffer s.hash_state)
+                                                     (B.loc_buffer s.tx)) h1 h3 new_hash_st;
+
+    lemma_transcript_bytes12 (G.reveal msg) (transcript s h0)
+
+let extend_hash13 s b p0 p1 msg =
+  let hash_st_opt = B.index s.hash_state 0ul in
+  match hash_st_opt with
+  | Some (| a, hash_st |) ->
+    let e_tx = B.index s.tx 0ul in
+    let prev_bytes = G.elift1 transcript_bytes e_tx in
+    let sub_b = B.sub b p0 (p1 - p0) in
+    assume (Seq.length (G.reveal prev_bytes) + UInt32.v (p1 - p0) < pow2 61);
+
+    let h0 = ST.get () in
+
+    let new_hash_st = IncHash.update a hash_st prev_bytes sub_b (p1 - p0) in
+
+    let h1 = ST.get () in
+
+    B.upd s.hash_state 0ul (Some (| a, new_hash_st |));
+
+    let e_tx = G.elift2_p extend_transcript13 e_tx msg in
+    B.upd s.tx 0ul e_tx;
+
+    let h3 = ST.get () in
+
+    //AR: this does not have a pattern, so need to call explicitly
+    IncHash.modifies_disjoint_preserves (B.loc_union (B.loc_buffer s.hash_state)
+                                                     (B.loc_buffer s.tx)) h1 h3 new_hash_st;
+
+    lemma_transcript_bytes13 (G.reveal msg) (transcript s h0)
 
 let extract_hash #a s tag =
   let hash_st_opt = B.index s.hash_state 0ul in
@@ -168,7 +230,4 @@ let extract_hash #a s tag =
 
     let h1 = ST.get () in
 
-    assume (Seq.length (G.reveal prev_bytes) < Spec.Hash.Definitions.max_input_length a);
-
-    assume (B.(loc_includes (loc_union (footprint s h1) (loc_buffer tag))
-                            (loc_union (IncHash.footprint hash_st h1) (loc_buffer tag))))
+    assume (Seq.length (G.reveal prev_bytes) < Spec.Hash.Definitions.max_input_length a)
