src/tls/HSL.Transcript.fsti
@@ -9,20 +9,35 @@ module List = FStar.List.Tot
 module HS = FStar.HyperStack
 module B = LowStar.Buffer
 
-module Hash = Hashing
-module HSM = HandshakeMessages
+open Parsers.Handshake13
+
+module HSM = Parsers.Handshake
+module HSM12 = Parsers.Handshake12
+module HSM13 = Parsers.Handshake13
 
 open HSL.Common
 
-#reset-options
-   "--log_queries --query_stats \
-    --using_facts_from 'Prims FStar LowStar -FStar.Reflection -FStar.Tactics -FStar.UInt128 -FStar.Math' \
-    --using_facts_from 'Mem HSL Types_s Words_s Spec.Hash.Definitions.bytes' \
-    --using_facts_from 'TLSError'"
+type bytes = Spec.Hash.Definitions.bytes
 
-let transcript_t = list HSM.hs_msg
-let transcript_bytes (t:transcript_t) : GTot hbytes =
-  List.fold_right_gtot t (fun x a -> Seq.append a (format_hs_msg x)) Seq.empty
+type alg = Spec.Hash.Definitions.hash_alg
+
+noeq type transcript_t =
+  | Transcript_nil: transcript_t
+  | Transcript_hello_server: h:list HSM.handshake -> transcript_t
+  | Transcript12: h:list HSM.handshake -> m:list HSM12.handshake12 -> transcript_t
+  | Transcript13: h:list HSM.handshake -> m:list HSM13.handshake13 -> transcript_t
+
+let transcript_bytes (t:transcript_t) : GTot bytes =
+  match t with
+  | Transcript_nil -> Seq.empty
+  | Transcript_hello_server h ->
+    List.fold_right_gtot h (fun x a -> Seq.append a (format_hs_msg x)) Seq.empty
+  | Transcript12 h m ->
+    Seq.append (List.fold_right_gtot h (fun x a -> Seq.append a (format_hs_msg x)) Seq.empty)
+               (List.fold_right_gtot m (fun x a -> Seq.append a (format_hs12_msg x)) Seq.empty)
+  | Transcript13 h m ->
+    Seq.append (List.fold_right_gtot h (fun x a -> Seq.append a (format_hs_msg x)) Seq.empty)
+               (List.fold_right_gtot m (fun x a -> Seq.append a (format_hs13_msg x)) Seq.empty)
 
 val state : Type0
 
@@ -34,7 +49,7 @@ val transcript : state -> HS.mem -> GTot transcript_t
 
 /// Hashing algorithm in use
 
-val hash_alg : state -> HS.mem -> GTot (option Hash.alg)
+val hash_alg : state -> HS.mem -> GTot (option alg)
 
 val invariant : state -> HS.mem -> prop
 
@@ -63,9 +78,9 @@ val create (r:Mem.rgn)
          fresh_loc (footprint s h1) h0 h1 /\
          r `region_includes` footprint s h1 /\
 	 hash_alg s h1 == None /\
-	 transcript s h1 == [])
+	 transcript s h1 == Transcript_nil)
 
-val set_hash_alg (a:Hash.alg) (s:state)
+val set_hash_alg (a:alg) (s:state)
   : ST unit
        (requires fun h ->
          invariant s h /\
@@ -79,42 +94,132 @@ val set_hash_alg (a:Hash.alg) (s:state)
                footprint s h1 == B.loc_union l (footprint s h0) /\
                region_of s `region_includes` footprint s h1))
 
-let extend_transcript (s:state) (msg:HSM.hs_msg) (h:HS.mem) : GTot transcript_t =
-  match hash_alg s h with
-  | None -> []
-  | Some _ -> msg :: transcript s h
+let can_extend_with_hsm (t:transcript_t) =
+  match t with
+  | Transcript_nil -> True
+  | Transcript_hello_server _ -> True
+  | _ -> False
 
-val extend_hash (s:state)
-                (b:B.buffer uint_8)
-                (p0:uint_32)
-                (p1:uint_32{p0 <= p1 /\ p1 <= B.len b})
-                (msg:G.erased HSM.hs_msg)
+let can_extend_with_hsm12 (t:transcript_t) =
+  match t with
+  | Transcript_hello_server _ -> True
+  | Transcript12 _ _ -> True
+  | _ -> False
+
+let can_extend_with_hsm13 (t:transcript_t) =
+  match t with
+  | Transcript_hello_server _ -> True
+  | Transcript13 _ _ -> True
+  | _ -> False
+
+let extend_transcript
+  (t:transcript_t)
+  (msg:HSM.handshake{can_extend_with_hsm t})
+  : GTot transcript_t
+  = match t with
+    | Transcript_nil -> Transcript_hello_server [msg]
+    | Transcript_hello_server msgs -> Transcript_hello_server (msg::msgs)
+
+let extend_transcript12
+  (t:transcript_t)
+  (msg:HSM12.handshake12{can_extend_with_hsm12 t})
+  : GTot transcript_t
+  = match t with
+    | Transcript_hello_server msgs -> Transcript12 msgs [msg]
+    | Transcript12 hmsgs msgs -> Transcript12 hmsgs (msg::msgs)
+
+let extend_transcript13
+  (t:transcript_t)
+  (msg:HSM13.handshake13{can_extend_with_hsm13 t})
+  : GTot transcript_t
+  = match t with
+    | Transcript_hello_server msgs -> Transcript13 msgs [msg]
+    | Transcript13 hmsgs msgs -> Transcript13 hmsgs (msg::msgs)
+
+unfold let extend_hash_pre_common
+  (s:state)
+  (b:B.buffer uint_8)
+  (h:HS.mem)
+  = invariant s h /\
+    B.live h b /\
+    B.loc_disjoint (B.loc_buffer b) (footprint s h) /\
+    Some? (hash_alg s h)
+
+unfold let extend_hash_post_common
+  (s:state)
+  (b:B.buffer uint_8)
+  (h0 h1:HS.mem)
+  = invariant s h1 /\
+    B.modifies (footprint s h1) h0 h1 /\
+    footprint s h1 == footprint s h0 /\
+    hash_alg s h1 == hash_alg s h0
+
+val extend_hash
+  (s:state)
+  (b:B.buffer uint_8)
+  (p0:uint_32)
+  (p1:uint_32)
+  (msg:G.erased HSM.handshake)
   : ST unit
        (requires fun h ->
-         invariant s h /\
-	 B.live h b /\
-	 B.loc_disjoint (B.loc_buffer b) (footprint s h) /\
+         extend_hash_pre_common s b h /\
+	 can_extend_with_hsm (transcript s h) /\
          valid_parsing (G.reveal msg) p0 p1 b h)
        (ensures (fun h0 _ h1 ->
-         invariant s h1 /\
-	 B.modifies (footprint s h1) h0 h1 /\
-         footprint s h1 == footprint s h0 /\
-         hash_alg s h1 == hash_alg s h0 /\
-         transcript s h1 == extend_transcript s (G.reveal msg) h0))
+         extend_hash_post_common s b h0 h1 /\
+         transcript s h1 == extend_transcript (transcript s h0) (G.reveal msg)))
 
-let buf_is_hash_of_b (a:Hash.alg) (buf:Hacl.Hash.Definitions.hash_t a) (h:HS.mem) (b:hbytes)
+val extend_hash12
+  (s:state)
+  (b:B.buffer uint_8)
+  (p0:uint_32)
+  (p1:uint_32)
+  (msg:G.erased HSM12.handshake12)
+  : ST unit
+       (requires fun h ->
+         extend_hash_pre_common s b h /\
+	 can_extend_with_hsm12 (transcript s h) /\
+         valid_parsing12 (G.reveal msg) p0 p1 b h)
+       (ensures (fun h0 _ h1 ->
+         extend_hash_post_common s b h0 h1 /\
+         transcript s h1 == extend_transcript12 (transcript s h0) (G.reveal msg)))
+
+val extend_hash13
+  (s:state)
+  (b:B.buffer uint_8)
+  (p0:uint_32)
+  (p1:uint_32)
+  (msg:G.erased HSM13.handshake13)
+  : ST unit
+       (requires fun h ->
+         extend_hash_pre_common s b h /\
+	 can_extend_with_hsm13 (transcript s h) /\
+         valid_parsing13 (G.reveal msg) p0 p1 b h)
+       (ensures (fun h0 _ h1 ->
+         extend_hash_post_common s b h0 h1 /\
+         transcript s h1 == extend_transcript13 (transcript s h0) (G.reveal msg)))
+
+let buf_is_hash_of_b (a:alg) (tag:Hacl.Hash.Definitions.hash_t a) (h:HS.mem) (b:bytes)
   = assume (Seq.length b < Spec.Hash.Definitions.max_input_length a);  //AR: need to sort this out
-    B.as_seq h buf == Spec.Hash.hash a b
+    admit ();  //AR: TODO: strange behavior with interleaving
+               //          verifying just the .fsti does not need this admit
+	       //          but when verifying the .fst, this definition does not verify
+	       //          my suspicion is some options going wrong
+    B.as_seq h tag == Spec.Hash.hash a b
 
-val extract_hash (#a:Hash.alg) (s:state) (tag:Hacl.Hash.Definitions.hash_t a)
-  : ST unit (fun h0 ->
-             invariant s h0 /\
-             hash_alg s h0 == Some a /\
-             B.live h0 tag /\
-             B.loc_disjoint (footprint s h0) (B.loc_buffer tag))
-            (fun h0 _ h1 ->
-             let open B in
-	     frame_state s h0 h1 /\
-	     invariant s h1 /\
-             modifies (loc_union (footprint s h1) (loc_buffer tag)) h0 h1 /\
-             buf_is_hash_of_b a tag h1 (transcript_bytes (transcript s h1)))
+val extract_hash
+  (#a:alg)
+  (s:state)
+  (tag:Hacl.Hash.Definitions.hash_t a)
+  : ST unit
+       (requires (fun h0 ->
+         invariant s h0 /\
+         hash_alg s h0 == Some a /\
+         B.live h0 tag /\
+         B.loc_disjoint (footprint s h0) (B.loc_buffer tag)))
+       (ensures (fun h0 _ h1 ->
+         let open B in
+	 frame_state s h0 h1 /\
+	 invariant s h1 /\
+         modifies (loc_union (footprint s h1) (loc_buffer tag)) h0 h1 /\
+         buf_is_hash_of_b a tag h1 (transcript_bytes (transcript s h1))))
